universes etc

src/Pipit.Exp.Causality.fst
@@ -656,7 +656,7 @@ let lemma_bigstep_total_v
   (#c: context t)
   (#a: t.ty)
   (rows: list (row c) { Cons? rows }) (e: exp t c a { causal e }):
-    t.ty_sem a =
+    v: t.ty_sem a { bigstep rows e v } =
   let (| v, _ |) = lemma_bigstep_total rows e in
   v
 
@@ -665,6 +665,17 @@ let lemma_bigsteps_total_vs
   (#c: context t)
   (#a: t.ty)
   (rows: list (row c)) (e: exp t c a { causal e }):
-    vs: list (t.ty_sem a) { List.Tot.length vs == List.Tot.length rows } =
+    vs: list (t.ty_sem a) { List.Tot.length vs == List.Tot.length rows /\ bigsteps rows e vs } =
   let (| vs, _ |) = lemma_bigsteps_total rows e in
   vs
+
+let lemma_bigstep_total_always
+  (#t: table)
+  (#c: context t)
+  (rows: list (row c)) (row1: row c) (e: exp t c t.propty { causal e }):
+  Lemma (requires (bigstep_always (row1 :: rows) e))
+    (ensures (lemma_bigstep_total_v (row1 :: rows) e == true))
+    [SMTPat (bigstep_always (row1 :: rows) e)] =
+  let v = lemma_bigstep_total_v (row1 :: rows) e in
+  // let (| v, hBS |) = lemma_bigstep_total (row1 :: rows) e in
+  bigstep_deterministic_squash (row1 :: rows) e v true
